src/basicmodal/syntax/soundness.lean
@@ -13,7 +13,7 @@ theorem soundness (AX : ctx) (φ : form) : prfK AX φ → global_sem_csq AX φ :
 begin
 intro h,
 induction h,
-{intros f v x h, rw forces_ctx at h,
+{intros f v h x, rw forces_ctx at h,
 specialize h h_φ x, have h1 := h h_h, 
 exact h1},
 {intros f v x h2 h3 h4, exact h3}, 
@@ -38,9 +38,9 @@ specialize h2 x' h4 h3, exact h2},
 specialize h_ih_hpq f v x h,
 specialize h_ih_hp f v x h,
 exact h_ih_hpq h_ih_hp}, 
-{intros f v x h1 y h2,
+{intros f v h1 x y h2,
 rw global_sem_csq at h_ih,
-specialize h_ih f v y h1, 
+specialize h_ih f v h1 y, 
 exact h_ih},
 end
 
